\begin{equation} 
S_{p_{contact}}^{x} &= m(\vect{q}_{|k})_{x}^{eq} \ddot{X}_{EE_{|k}}^{\vect{x}} (\vect{X}_{x_{|k}}^{*} - \vect{X}_{x_{|k}}) \vect{x},
\label{eq:hwcmputeEpx}
\end{equation}
\begin{equation} 
\textnormal{With: } 
\ddot{X}_{EE_{|k}}^{\vect{x}} = (\dot{J}(\vect{q}_{|k})_{EE} \vect{\dot{q}}_{|k} + J(\vect{q}_{|k})_{EE} \vect{\ddot{q}}_{|k}^{c}) \vect{x}, \\
\textnormal{And: }
\vect{\ddot{q}}_{|k}^{c}} =  M(\vect{q}_{|k})^{-1}(\vect{\tau}_{|k}^{c}-\vect{b}(\vect{q}_{|k},\vect{\dot{q}}_{|k}))
\label{eq:vefef_futur}
\end{equation}
\begin{equation} 
\textnormal{And: }
\vect{\ddot{q}}_{|k}^{c}} =  M(\vect{q}_{|k})^{-1}(\vect{\tau}_{|k}^{c}-\vect{b}(\vect{q}_{|k},\vect{\dot{q}}_{|k}))
\label{eq:vefef_futurhrth}
\end{equation}



M(\vect{q}_{|k}) \vect{\ddot{q}}_{|k}^{c} + \vect{b}(\vect{q}_{|k},\vect{\dot{q}}_{|k}) = \vect{\tau}_{|k}^{c}



\usepackage{style/uomthesis}

\usepackage{geometry}
\newcounter{mylabelcounter}


 \geometry{
 a4paper,
 total={170mm,257mm},
 left=20mm,
 top=20mm,
 }